verif/btrees/verif_getrecord.v
@@ -64,7 +64,7 @@ Proof.
       rep_omega. destruct H. 
       clear - SUBNODE H. hnf in H. simpl in H.
       destruct (Znth_option i le) eqn:?H; try contradiction.
-       apply nth_entry_le_some in H0. rep_omega. }
+       apply Znth_option_some in H0. rep_omega. }
     { forward.                  (* skip *)
       entailer!. unfold normc. unfold n. simpl.
       rewrite (proj2 (Z.eqb_neq i (Zlength le))); auto. contradict H4. f_equal; auto. }
@@ -90,11 +90,11 @@ Proof.
       clear - H4.
       hnf in H4; simpl in H4.
       destruct (Znth_option normi nle) eqn:?H; try contradiction.
-      apply nth_entry_le_some in H; auto.
+      apply Znth_option_some in H; auto.
    }
-    apply nth_entry_le_in_range in ZNTH.
+    apply Znth_option_in_range in ZNTH.
     destruct ZNTH as [e ZNTH].
-    assert(ZTL: nth_entry_le normi nle = Some e) by auto.
+    assert(ZTL: Znth_option normi nle = Some e) by auto.
     apply Znth_to_list' with (endle:=ent_end0) in ZTL.
     assert(INTEGRITY: subnode normn root) by (rewrite HNORMN; auto).
     apply H3 in INTEGRITY. rewrite HNORMN in INTEGRITY.
@@ -106,14 +106,14 @@ Proof.
     2: eauto.
     
     destruct INTEGRITY as [k [v [x HE]]].
-    assert(LESPLIT: nth_entry_le normi nle = Some e) by auto.
+    assert(LESPLIT: Znth_option normi nle = Some e) by auto.
     apply le_iter_sepcon_split in LESPLIT. rewrite LESPLIT. Intros.
     assert (H99: 0 <= normi < Fanout). {
      pose proof (H2 _ SUBNODE').
      apply node_wf_numKeys in H6. simpl in H6. clear - H6 H4.
       hnf in H4; simpl in H4.
       destruct (Znth_option normi nle) eqn:?H; try contradiction.
-      apply nth_entry_le_some in H. rep_omega. 
+      apply Znth_option_some in H. rep_omega. 
     }
     
     forward.                    (* t'6=t'4->entries[t'5]->ptr.record *)
@@ -127,7 +127,7 @@ Proof.
     fold Inhabitant_entry_val_rep. rewrite ZTL. entailer!.
     fold Inhabitant_entry_val_rep. rewrite ZTL. entailer!.
     { simpl. unfold RL_GetRecord. fold n. fold c. fold r. rewrite HNORMC.
-      unfold getCVal. simpl. unfold nth_entry_le in ZNTH; rewrite ZNTH. auto. }
+      unfold getCVal. simpl. rewrite ZNTH. auto. }
     rewrite <- HNORMC. unfold normalize. unfold c. unfold n. simpl. unfold r. cancel.
     rewrite <- ?Vptrofs_repr_Vlong_repr by auto. cancel.
 Qed.
